First step: - introduce mock deref_loc and assign_loc predicates, with traces - break CompCert C's evaluation of op= and ++ in two steps,   each with single-event traces - introduce Stuckstate and take advantage of it to lighten the need for   "safe" hypothesis in Cstrategy - add fail-in-the-middle rules for op= and ++ in Cstrategy - update Cstrategy (fully) and Clight, SimplExpr (lightly).
git-svn-id: https://yquem.inria.fr/compcert/svn/compcert/branches/volatiles@1795 fca1b0fc-160b-0410-b1d3-a4f43f01ea2e

cfrontend/Clight.v
@@ -179,6 +179,30 @@ Definition empty_env: env := (PTree.empty (block * type)).
 
 Definition temp_env := PTree.t val.
 
+(** [load_value_of_type ty m b ofs] computes the value of a datum
+  of type [ty] residing in memory [m] at block [b], offset [ofs].
+  If the type [ty] indicates an access by value, the corresponding
+  memory load is performed.  If the type [ty] indicates an access by
+  reference, the pointer [Vptr b ofs] is returned. *)
+
+Definition load_value_of_type (ty: type) (m: mem) (b: block) (ofs: int) : option val :=
+  match access_mode ty with
+  | By_value chunk => Mem.loadv chunk m (Vptr b ofs)
+  | By_reference => Some (Vptr b ofs)
+  | By_nothing => None
+  end.
+
+(** Symmetrically, [store_value_of_type ty m b ofs v] returns the
+  memory state after storing the value [v] in the datum
+  of type [ty] residing in memory [m] at block [b], offset [ofs].
+  This is allowed only if [ty] indicates an access by value. *)
+
+Definition store_value_of_type (ty_dest: type) (m: mem) (loc: block) (ofs: int) (v: val) : option mem :=
+  match access_mode ty_dest with
+  | By_value chunk => Mem.storev chunk m (Vptr loc ofs) v
+  | By_reference => None
+  | By_nothing => None
+  end.
 
 (** Selection of the appropriate case of a [switch], given the value [n]
   of the selector expression. *)
